Convergence proof wip

inductive_proof/Last-writer-wins_register/App.fst
@@ -44,7 +44,7 @@ let concrete_merge (lca s1 s2:concrete_st)
   : Pure concrete_st
          (requires (exists l1 l2. apply_log lca l1 == s1 /\ apply_log lca l2 == s2))
          (ensures (fun _ -> True)) =
-  if fst s1 < fst s2 then s2 else s1
+  if fst s1 = fst s2 then lca else if fst s1 < fst s2 then s2 else s1
 
 let rec lem_foldl (s:concrete_st) (l:log)
   : Lemma (requires true)
@@ -215,18 +215,45 @@ let merge_pre (lca s1 s2:concrete_st) =
   fst s1 >= fst lca /\ fst s2 >= fst lca /\
   (fst s1 = fst s2 ==> s1 = s2)
 
-#push-options "--z3rlimit 100"
-let convergence1 (lca s1 s2 s1':st) (o:op_t)
-  : Lemma (requires s1 == do_st s1' o /\
-                    consistent_branches lca s1 s2 /\
-                    consistent_branches lca s1' s2 /\
-                    (exists l1 l2. apply_log (v_of s1') l1 == (concrete_merge (v_of lca) (v_of s1') (v_of s2)) /\ 
-                              apply_log (v_of s1') l2 == v_of s1))
-          (ensures eq (concrete_merge (v_of lca) (v_of s1) (v_of s2)) 
-                      (concrete_merge (v_of s1') (concrete_merge (v_of lca) (v_of s1') (v_of s2)) (v_of s1))) = 
-  assume (fst o > fst (v_of s1')); //assumption
-  assume (fst (v_of s1) <> fst (v_of s2)); //assumption
-  ()
+let do_prop (s:concrete_st) (o:op_t) 
+  : Lemma (fst (do s o) = fst o) = ()
+
+let concrete_merge1 (lca s1 s2:concrete_st) : Tot concrete_st =
+  if fst s1 < fst s2 then s2 else s1
+
+#push-options "--z3rlimit 300"
+let convergence1 (lca s1' s2:st) (o:op_t)
+  : Lemma (requires is_prefix (ops_of lca) (ops_of s1') /\
+                    (forall id. mem_id id (ops_of s1') ==> fst o > id))
+          (ensures eq (concrete_merge1 (v_of lca) (do (v_of s1') o) (v_of s2)) 
+                      (concrete_merge1 (v_of s1') (do (v_of s1') o) (concrete_merge1 (v_of lca) (v_of s1') (v_of s2))))
+          (decreases %[length (ops_of s1')]) = 
+  do_prop (v_of s1') o;
+  if ops_of s1' = ops_of lca then 
+    (if fst (v_of s1') < fst o then () //done
+     else if fst (v_of s1') > fst o then 
+       (if length (ops_of lca) = 0 then () //done 
+        else 
+          (let l' = inverse_st lca in
+           let pre, lastop = un_snoc (ops_of lca) in
+           lemma_append_count_assoc_fst pre (create 1 lastop);
+           assert (mem_id (fst lastop) (ops_of s1'));
+           assert (v_of s1' == (fst lastop, snd lastop)); 
+           assert (fst (v_of s1') < fst o); //proof by contradiction
+           ())) //done
+     else ()) //done
+  else 
+    (if fst (v_of s1') < fst o then () //done
+     else if fst (v_of s1') > fst o then 
+       (let s1'' = inverse_st s1' in
+        let pre, lastop = un_snoc (ops_of s1') in
+        lemma_append_count_assoc_fst pre (create 1 lastop);
+        assert (is_prefix (ops_of s1') (snoc (ops_of s1') o));
+        assert (mem_id (fst lastop) (ops_of s1')); 
+        assert (v_of s1' == (fst lastop, snd lastop));
+        assert (fst (v_of s1') < fst o); //proof by contradiction
+        ()) //done
+     else ()) //done
 
 let convergence2 (lca s2 s3 lca' s1':st)
   : Lemma (requires consistent_branches lca' s3 s1' /\
